% arara: pdflatex


\documentclass[12pt, letterpaper]{article}
\usepackage[utf8]{inputenc}
\usepackage{amsmath}


\title{Relativitization}

\author{Adriankhl}


\begin{document}

\begin{titlepage}
\maketitle
\end{titlepage}

\section{Photon rocket}

Photon 4-momentum: $P_{ph}$, object initial 4-momentum $P_i = (\gamma_i m_i c, \gamma_i m_i \overrightarrow{v}) $,
object final 4-momentum $P_f = (\gamma_f m_f c, \gamma_f m_f \alpha \hat{u})$. Let $m_f = m_i - \Delta m$.

\begin{align*}
  P_{ph} &= P_i - P_f \\
  P_{ph}^2 &= P_i^2 + P_f^2 - 2 P_i \cdot P_f \\
  0 &= (m_i c)^2 + (m_f c)^2 - 2 \gamma_i \gamma_f m_i m_f ( c^2 - \alpha \overrightarrow{v} \cdot \hat{u}) \\
  (m_i c)^2 + (m_f c)^2 &= \frac{2 \gamma_i m_i m_f}{\sqrt{1 - \alpha^2 / c^2}} ( c^2 - \alpha \overrightarrow{v} \cdot \hat{u}) \\
  \left(\frac{(m_i c)^2 + (m_f c)^2}{2 \gamma_i m_i m_f}\right)^2 &= \frac{(c^2 - \alpha \overrightarrow{v} \cdot \hat{u})^2}{1 - \alpha^2 / c^2} \\
  \left(\frac{(m_i c)^2 + (m_f c)^2}{2 \gamma_i m_i m_f}\right)^2 (1 - \alpha^2 / c^2) &= c^4 - 2 c^2 \alpha \overrightarrow{v} \cdot \hat{u} + \alpha^2 (\overrightarrow{v} \cdot \hat{u})^2 \\
\end{align*}

\begin{equation*}
  ((\overrightarrow{v} \cdot \hat{u})^2 + \left(\frac{(m_i)^2 + (m_f)^2}{2 \gamma_i m_i m_f}\right)^2 c^2) \alpha ^2 + (- 2 c^2 \overrightarrow{v} \cdot \hat{u}) \alpha + c^4 \left(1 - \left(\frac{(m_i)^2 + (m_f)^2}{2 \gamma_i m_i m_f}\right)^2 \right) = 0
\end{equation*}

If $|\overrightarrow{v}| = 0$

\begin{align*}
  (\left(\frac{(m_i)^2 + (m_f)^2}{2 m_i m_f}\right)^2 c^2) \alpha^2 + c^4 \left(1 - \left(\frac{(m_i)^2 + (m_f)^2}{2 m_i m_f}\right)^2 \right) &= 0 \\
  ((m_i)^2 + (m_f)^2)^2 \alpha^2 + c^2 ((2 m_i m_f)^2 - (m_i)^4 - 2 (m_i)^2 (m_f)^2 - (m_f)^4) &= 0 \\
  ((m_i)^2 + (m_f)^2)^2 \alpha^2 - c^2 ((m_i)^4 - 2 (m_i)^2 (m_f)^2 + (m_f)^4) &= 0 \\
  ((m_i)^2 + (m_f)^2)^2 \alpha^2 - c^2 ((m_i)^2 - (m_f)^2)^2 &= 0
\end{align*}

\end{document}
